Test/Semantics/Dynamic.v
@@ -127,60 +127,105 @@ Definition WellTyped__E
   : (TypedExpr T V)-indexedPropFunctor
   := (WellTyped__Bool).
 
-Definition SourceExpr := Bool + If1 + Unit.
-Definition TargetExpr := Bool + If2 + Unit.
-Definition Value := Bool + Stuck + Unit.
+(* Definition SourceExpr := Bool + If1 + Unit. *)
+(* Definition TargetExpr := Bool + If2 + Unit. *)
+(* Definition Value := Bool + Stuck + Unit. *)
 
-Definition EvalRelation__Source
-  : (WellFormedValue SourceExpr * WellFormedValue Value)-indexedPropFunctor
-  := (EvalRelation__Bool + EvalRelation__If1 + EvalRelation__Unit)%IndexedSum1.
+(* Definition EvalRelation__Source *)
+(*   : (WellFormedValue SourceExpr * WellFormedValue Value)-indexedPropFunctor *)
+(*   := (EvalRelation__Bool + EvalRelation__If1 + EvalRelation__Unit)%IndexedSum1. *)
 
-Definition EvalRelation__Target
-  : (WellFormedValue TargetExpr * WellFormedValue Value)-indexedPropFunctor
-  := (EvalRelation__Bool + EvalRelation__If2 + EvalRelation__Unit)%IndexedSum1.
+(* Definition EvalRelation__Target *)
+(*   : (WellFormedValue TargetExpr * WellFormedValue Value)-indexedPropFunctor *)
+(*   := (EvalRelation__Bool + EvalRelation__If2 + EvalRelation__Unit)%IndexedSum1. *)
 
-Definition removeUnaryIfs'
-           (e : WellFormedValue SourceExpr)
-  : WellFormedValue TargetExpr
-  := removeUnaryIfs (L := SourceExpr) (V := TargetExpr) (proj1_sig e).
+(* Definition removeUnaryIfs' *)
+(*            (e : WellFormedValue SourceExpr) *)
+(*   : WellFormedValue TargetExpr *)
+(*   := removeUnaryIfs (L := SourceExpr) (V := TargetExpr) (proj1_sig e). *)
 
-Theorem test
-  : removeUnaryIfs' (if1 (boolean true) unit) = if2 (boolean true) unit unit.
-Proof.
-  reflexivity.
-Qed.
+(* Theorem test *)
+(*   : removeUnaryIfs' (if1 (boolean true) unit) = if2 (boolean true) unit unit. *)
+(* Proof. *)
+(*   reflexivity. *)
+(* Qed. *)
 
 Variant ForRemoveUnaryIfsCorrectness := .
+
+Delimit Scope Prod1_scope with Prod1.
+Open Scope Prod1_scope.
+
+Variant Prod1 (F G : Set -> Set) (A : Set) : Set :=
+| prod1 : F A -> G A -> (F * G)%Sum1 A
+where
+"F * G" := (Prod1 F G) : Prod1_scope.
+
+Arguments prod1 {F G A}.
+
+Global Instance Functor_Prod1
+       {F G} `{Functor F} `{Functor G}
+  : Functor (F * G)
+  | 0 :=
+  {|
+    fmap := fun A B f '(prod1 fa ga) => prod1 (fmap f fa) (fmap f ga);
+  |}.
+
+Global Instance FunctorLaws_Prod1 F G `{FunctorLaws F} `{FunctorLaws G}
+  : FunctorLaws (Prod1 F G).
+Proof.
+  constructor.
+  {
+    move => A [] f g /=.
+    do 2 rewrite fmapId //.
+  }
+  {
+    move => A B C f g [] fa ga /=.
+    do 2 rewrite fmapFusion //.
+  }
+Qed.
+
+(*
+NOTE:
+
+I was trying to do a [WellFormedProofAlgebra2], that took a (Source * Value)
+pair and rebuilt it, but you end up wanting a product functor, and then you'd
+end up with [A <= A * B] constraints, which might not be true or not be worth it.
+
+It seems like it might be better to do a [WellFormedProofAlgebra] where you only
+change one of the two elements ofthe pair at the time, kind of like if you do
+induction one variable at a time rather than induction on the pair.
+
+Probably want to do induction on the source term, with the value universally
+quantified in the output.
+ *)
 
 Definition AbstractCorrectnessStatement
            {S T V}
            `{FunctorLaws S} `{FunctorLaws T} `{FunctorLaws V}
-           (EvalRelation__Source : (WellFormedValue S * WellFormedValue V)-indexedPropFunctor)
-           (EvalRelation__Target : (WellFormedValue T * WellFormedValue V)-indexedPropFunctor)
+           (EvalRelation__Source : (Fix S * Fix V)-indexedPropFunctor)
+           (EvalRelation__Target : (Fix T * Fix V)-indexedPropFunctor)
            `{removeUnaryIfs__S : forall {R}, MixinAlgebra S R (WellFormedValue T)}
            (recRemoveUnaryIfs : WellFormedValue S -> WellFormedValue T)
-           (ev : Fix S * Fix V)
-           (UP'__ev : FoldUP' (fst ev) /\ FoldUP' (snd ev))
+           (s : Fix S)
+           (UP'__s : FoldUP' s)
   : Prop
-  := IndexedFix EvalRelation__Source
-                ( exist _ (fst ev) (proj1 UP'__ev),
-                  exist _ (snd ev) (proj2 UP'__ev)
-                ) ->
-     IndexedFix EvalRelation__Target
-                ( removeUnaryIfs__S recRemoveUnaryIfs (unwrapUP' (fst ev)),
-                  wrapUP' (unwrapUP' (snd ev))
-                ).
+  := forall (v : Fix V),
+    IndexedFix EvalRelation__Source (s, v) ->
+    IndexedFix EvalRelation__Target
+               ( proj1_sig (removeUnaryIfs__S recRemoveUnaryIfs (unwrapUP' s)),
+                 v
+               ).
 
 Definition Correctness__ProofAlgebra
            {S T V}
            `{FunctorLaws S} `{FunctorLaws T} `{FunctorLaws V}
-           (EvalRelation__Source : (WellFormedValue S * WellFormedValue V)-indexedPropFunctor)
-           (EvalRelation__Target : (WellFormedValue T * WellFormedValue V)-indexedPropFunctor)
+           (EvalRelation__Source : (Fix S * Fix V)-indexedPropFunctor)
+           (EvalRelation__Target : (Fix T * Fix V)-indexedPropFunctor)
            `{RemoveUnaryIfs__S : forall {R}, ProgramAlgebra ForRemoveUnaryIfs S R (WellFormedValue T)}
   := forall recRemoveUnaryIfs,
     ProofAlgebra ForRemoveUnaryIfsCorrectness
-                 SourceExpr
-                 (sig (UniversalPropertyP2
+                 S
+                 (sig (UniversalPropertyP
                          (AbstractCorrectnessStatement
                             (removeUnaryIfs__S := fun _ => programAlgebra' RemoveUnaryIfs__S)
                             EvalRelation__Source
@@ -192,110 +237,52 @@ Definition Correctness__ProofAlgebra
 Lemma Correctness
       {S T V}
       `{FunctorLaws S} `{FunctorLaws T} `{FunctorLaws V}
-      (EvalRelation__Source : (WellFormedValue S * WellFormedValue V)-indexedPropFunctor)
-      (EvalRelation__Target : (WellFormedValue T * WellFormedValue V)-indexedPropFunctor)
+      (EvalRelation__Source : (Fix S * Fix V)-indexedPropFunctor)
+      (EvalRelation__Target : (Fix T * Fix V)-indexedPropFunctor)
       `{RemoveUnaryIfs__S : forall {R}, ProgramAlgebra ForRemoveUnaryIfs S R (WellFormedValue T)}
-      (correctness__ProofAlgebra : Correctness__ProofAlgebra EvalRelation__Source EvalRelation__Target)
+      `{! WellFormedMendlerAlgebra (@RemoveUnaryIfs__S)}
+      (correctness__ProofAlgebra :
+         Correctness__ProofAlgebra EvalRelation__Source EvalRelation__Target)
       (WF_eval_Soundness_alg_F :
          forall recRemoveUnaryIfs,
-           WellFormedProofAlgebra2 (correctness__ProofAlgebra recRemoveUnaryIfs)
+           WellFormedProofAlgebra (correctness__ProofAlgebra recRemoveUnaryIfs)
       )
-  : forall (ev : WellFormedValue SourceExpr * WellFormedValue Value),
-    IndexedFix EvalRelation__Source
-               ( _, _
-               ) ->
-    IndexedFix EvalRelation__Target
-               ( removeUnaryIfs _, _
-               ).
-
-Theorem removeUnaryIfsCorrectness
-  : forall e v,
-    IndexedFix EvalRelation__Source (e, v) ->
-    IndexedFix EvalRelation__Target (removeUnaryIfs e, v).
+  : forall (s : Fix S)
+      (v : Fix V),
+    FoldUP' s ->
+    IndexedFix EvalRelation__Source (s, v) ->
+    IndexedFix EvalRelation__Target (proj1_sig (removeUnaryIfs s), v).
 Proof.
-  move => e v S.
-
-
-  pose proof @Induction2.
-
-
-  apply (Induction2 ().
-
-  apply iWrapFix.
-  case : (iUnwrapFix (e, v) S) => [ [ | ] |  ].
-
-  {
-    (* for some reason we need the @ to help type class resolution... *)
-    elim / @EvalInversionClear__Bool => b [] <- <- .
-    left.
-    left.
-    apply Bool.BoolValue.
-  }
-
-  {
-    elim / @EvalInversionClear__If1.
-
-    {
-      move => c t t' E__c E__t [] <- <- .
-      left.
-      right.
-      apply If2True.
-
-      {
-        apply iWrapFix.
-        case : (iUnwrapFix (c, boolean true) E__c) => [ [ | ] | ].
-
-        {
-          elim / @EvalInversionClear__Bool => b.
-          rewrite [@boolean]lock.
-          move => [].
-          unlock.
-          move => <- [] EQ.
-
-          (* can't find a nicer way of making this inversion happen *)
-          pose proof (wrapF_inversion' (E := Value) (boolean b) (boolean true) EQ) as EQ'.
-          move : EQ EQ' => _ [] ->.
-
-          left.
-          left.
-          apply Bool.BoolValue.
-        }
-
-        {
-          elim / @EvalInversionClear__If1.
-
-          {
-            move =>
-          }
-
-          admit.
-        }
-        {
-          admit.
-        }
-      }
-      {
-        admit.
-      }
-    }
-    {
-      case : (iUnwrapFix (c, boolean false) H) => [ [E | E] | E ].
-      {
-        inversion E.
-        left.
-        right.
-        constructor.
-        {
-          apply iWrapFix.
-
-        }
-      }
-      admit.
-    }
-  }
-  {
-    inversion_clear E.
-    right.
-    constructor.
-  }
+  move => s v UP'__s E__S.
+  rewrite <- (wrapUP'_unwrapUP' s) => //.
+  rewrite /= / removeUnaryIfs / mendlerFold / wrapF.
+  erewrite wellFormedMendlerAlgebra.
+  elim (
+      Induction
+        (PA := correctness__ProofAlgebra (fun s => removeUnaryIfs (proj1_sig s)))
+        _
+        _
+    ) => ? C.
+  apply : C => //.
 Qed.
+
+(* Let's instantiate it *)
+
+Definition SourceExpr := Bool + If1 + Unit.
+Definition TargetExpr := Bool + If2 + Unit.
+Definition Value := Bool + Stuck + Unit.
+
+Definition EvalRelation__Source
+  : (Fix SourceExpr * Fix Value)-indexedPropFunctor
+  := (EvalRelation__Bool + EvalRelation__If1 + EvalRelation__Unit)%IndexedSum1.
+
+Definition EvalRelation__Target
+  : (Fix TargetExpr * Fix Value)-indexedPropFunctor
+  := (EvalRelation__Bool + EvalRelation__If2 + EvalRelation__Unit)%IndexedSum1.
+
+Definition S' := If1.
+Definition T' := BoolType.
+Definition V' := If2.
+
+(* Definition CorrectnessInstantiation *)
+(*   := Correctness *)
