shell.nix
@@ -1,10 +1,14 @@
 { nixpkgs ? import <nixpkgs> {}
 }:
 with nixpkgs;
+let
+  coq = coq_8_9;
+  coqPackages = coqPackages_8_9;
+in
 mkShell {
   buildInputs = [
-    coq_8_9
-    coqPackages_8_9.coq-ext-lib
+    coq
+    coqPackages.coq-ext-lib
   ];
   COQBIN = "";
   name = "extensible-nanopass-compiler";
